\appendix
\section{Simplifying $z_2$'s inequalities for Case II.A.}
We have
\begin{align*}
 n - \Delta + \ell \leq & \Delta + (m - \ell) & \text{and} \\
 n - \Delta + \ell \leq & \Delta + 1 + \ell
\end{align*}
\begin{center}or\end{center}
\begin{align*}
 n - \Delta + 1 + m - \ell \leq & \Delta + (m - \ell) & \text{and} \\
 n - \Delta + 1 + m - \ell \leq & \Delta + 1 + \ell
\end{align*}
These can be simplified further with a bit of algebra:
\begin{align*}
 n-m +2\ell \leq & 2 \Delta & \text{and} \\
 n-1 \leq        & 2\Delta
\end{align*}
or
\begin{align*}
 n + 1 \leq         & 2 \Delta & \text{and} \\
 n + m - 2\ell \leq & 2 \Delta
\end{align*}

These inequalites are of the form
\begin{align*}
 n-x \leq & 2 \Delta & \text{and} \\
 n-1 \leq & 2\Delta
\end{align*}
\begin{center}or\end{center}
\begin{align*}
 n + x \leq & 2 \Delta & \text{and} \\
 n + 1 \leq & 2 \Delta
\end{align*}

Where $x = m -2\ell$.

Supposing $x\geq 0$, we have
\begin{align*}
 n-x \leq & n+x \leq 2 \Delta & \text{and} \\
 n-1 \leq & n+1 \leq 2\Delta
\end{align*}

Whereas if $x <0$, then from assumption A we must have $m-2\ell = -1$, so that
our constraints reduce to
\begin{align*}
 n+1 \leq & 2 \Delta & \text{and} \\
 n-1 \leq & 2 \Delta
\end{align*}

\newpage
\section{Simplifying $z_2$'s inequalities for Case II.B.}

We have
\begin{align*}
 n - \Delta + \ell \leq & \Delta + (m - \ell) & \text{and} \\
 n - \Delta + \ell \leq & \Delta + 1 + \ell
\end{align*}
\begin{center}or\end{center}
\begin{align*}
 n - \Delta + 1 + m - \ell \leq & \Delta + (m - \ell) & \text{and} \\
 n - \Delta + 1 + m - \ell \leq & \Delta + 1 + \ell
\end{align*}
These can be simplified further with a bit of algebra:
\begin{align*}
 n-m+2\ell \leq & 2 \Delta & \text{and} \\
 n-1 \leq       & 2\Delta
\end{align*}
or
\begin{align*}
 n+1 \leq        & 2 \Delta & \text{and} \\
 n+m-2\ell  \leq & 2 \Delta
\end{align*}

These inequalites are of the form
\begin{align*}
 n-x \leq & 2 \Delta & \text{and} \\
 n-1 \leq & 2\Delta
\end{align*}
\begin{center}or\end{center}
\begin{align*}
 n + 1 \leq & 2 \Delta & \text{and} \\
 n + x \leq & 2 \Delta
\end{align*}

Where $x = m -2\ell$. Now since assumption B gives $m - 2\ell \leq -1$, we
see that
\begin{align*}
 n-1 \leq & n-x \leq 2 \Delta \\
          & \text{or}         \\
 n+x \leq & n+1 \leq 2 \Delta
\end{align*}
